refactoring and adding examples

ProofWidgets/Demos/RefreshComponent.lean
@@ -2,20 +2,22 @@ import ProofWidgets.Component.RefreshComponent
 import ProofWidgets.Component.HtmlDisplay
 import ProofWidgets.Component.OfRpcMethod
 import ProofWidgets.Component.Panel.SelectionPanel
-import ProofWidgets.Demos.RefreshComponent.CancelToken
 
 /-!
-This file showcases the `RefreshComponent` using some basic examples
+This file showcases the `RefreshComponent` using some basic examples.
+
+We use `dbg_trace` to help see which Lean processes are active at any time.
 -/
 
 open Lean.Widget ProofWidgets RefreshComponent Jsx Lean Server
+
 
 /-! Example 1: Counting up to 10 -/
 
 partial def countToTen : CoreM Html := do
   mkRefreshComponentM (.text "Let's count to ten!!!") (count 0)
 where
-  count (n : Nat) : RefreshT CoreM Unit := refreshM do
+  count (n : Nat) : CoreM (RefreshStep CoreM) := do
     IO.sleep 1000
     dbg_trace "counted {n}"
     Core.checkSystem "count to ten"
@@ -28,10 +30,11 @@ where
 #html countToTen
 
 -- Here, we duplicate the widget using the same underlying computation
-#html (do let x ← countToTen; return <span>{x}{x}</span>)
+-- #html (do let x ← countToTen; return <span>{x}<br/>{x}</span>)
 
 -- Here, we duplicate the widget and duplicate the underlying computation
-#html (return <span>{← countToTen}{← countToTen}</span>)
+-- #html (return <span>{← countToTen}<br/>{← countToTen}</span>)
+
 
 
 /-! Example 2: print the selected expressions one by one in an infinite loop -/
@@ -39,11 +42,8 @@ where
 @[server_rpc_method]
 partial def cycleSelections (props : PanelWidgetProps) : RequestM (RequestTask Html) :=
   RequestM.asTask do
-    let cancelTk ← IO.CancelToken.new
-    if let some oldTk ← globalCancelToken.swap cancelTk then
-      oldTk.set
     let some goal := props.goals[0]? | return .text "there are no goals"
-    mkGoalRefreshComponent goal cancelTk (.text "loading...") do refreshM do
+    mkGoalRefreshComponent goal (.text "loading...") do
       let args ← props.selectedLocations.mapM (·.saveExprWithCtx)
       if h : args.size ≠ 0 then
         have : NeZero args.size := ⟨h⟩
@@ -51,30 +51,84 @@ partial def cycleSelections (props : PanelWidgetProps) : RequestM (RequestTask H
       else
         return .last <| .text "please select some expression"
 where
-  loop (args : Array ExprWithCtx) (i : Fin args.size) : MetaM (RefreshResult MetaM) := do
-    Core.checkSystem "cycleSelections"
-    return .cont (<InteractiveCode fmt={← args[i].runMetaM Widget.ppExprTagged}/>) do refreshM do
-    IO.sleep 1000
-    Core.checkSystem "cycleSelections"
-    have : NeZero args.size := ⟨by cases i; grind⟩
-    loop args (i + 1)
+  loop (args : Array ExprWithCtx) (i : Fin args.size) : MetaM (RefreshStep MetaM) := do
+    return .cont <InteractiveCode fmt={← args[i].runMetaM Widget.ppExprTagged}/> do
+      dbg_trace "cycled through expression {i}"
+      IO.sleep 1000
+      Core.checkSystem "cycleSelections"
+      have : NeZero args.size := ⟨by cases i; grind⟩
+      loop args (i + 1)
 
 @[widget_module]
-def cylceComponent : Component PanelWidgetProps :=
+def cycleComponent : Component PanelWidgetProps :=
   mk_rpc_widget% cycleSelections
 
--- show_panel_widgets [cylceComponent, cylceComponent]
-show_panel_widgets [cylceComponent]
-example : 1 + 2 + 3 = 6 ^ 1 := by -- place your cursor here and select some expressions
+elab stx:"cycleSelections" : tactic => do
+  Widget.savePanelWidgetInfo (hash cycleComponent.javascript) (pure <| json% {}) stx
+
+-- show_panel_widgets [cycleComponent, cycleComponent]
+example : 1 + 2 + 3 = 6 ^ 1 := by
+  cycleSelections -- place your cursor here and select some expressions
   rfl
 -- If you activate the widget multiple times, then thanks to the global cancel token ref,
--- All but one of the widget computations will say `This component was cancelled`.
+-- all but one of the widget computations will say `This component was cancelled`.
 
 
-/-! Example 4: compute the fibonacci numbers, and show the results incrementally. -/
 
-def slowFibo (n : Nat) : Nat :=
-  match n with
-  | 0 => 0
-  | 1 => 1
-  | n + 2 => slowFibo n + slowFibo (n + 1)
+/-! Example 3: compute the fibonacci numbers from 400000 to 400040, in parallel,
+and show the results as they come up. -/
+
+def fibo (n : Nat) : Nat := Id.run do
+  let mut (a, b) := (0, 1)
+  for _ in 0...n do
+    (a, b) := (b, a + b)
+  return a
+
+structure FiboState where
+  pending : Array (Nat × Task Html)
+  results : Array (Nat × Html) := #[]
+
+def FiboState.update (s : FiboState) : BaseIO FiboState := do
+  let mut results := s.results
+  let mut pending := #[]
+  for (n, t) in s.pending do
+    if ← IO.hasFinished t then
+      results := results.push (n, t.get)
+    else
+      pending := pending.push (n, t)
+  results := results.insertionSort  (·.1 < ·.1)
+  return { results, pending }
+
+def FiboState.render (s : FiboState) (t : Option Nat := none) : Html :=
+  let header := match t with
+    | some t => s!"Finished in {t}ms"
+    | none => "Computing Fibonacci numbers ⏳";
+  <details «open»={true}>
+    <summary className="mv2 pointer">
+      {.text header}
+    </summary>
+    {Html.element "ul" #[("style", json% { "padding-left" : "30px"})] (s.results.map (·.2))}
+  </details>
+
+def generateFibo (n : Nat) : Html :=
+  <li>{.text s!"the {n}-th Fibonacci number has {(fibo n).log2} binary digits."}</li>
+
+partial def FiboWidget : CoreM Html := do
+  mkRefreshComponentM (.text "loading...") do
+    IO.sleep 1 -- If we don't wait 1ms first, the infoview lags too much.
+    let pending := (400000...=400040).toArray.map fun n => (n, Task.spawn fun _ => generateFibo n)
+    let t0 ← IO.monoMsNow
+    loop t0 { pending }
+where
+  loop (t0 : Nat) (s : FiboState) : CoreM (RefreshStep CoreM) := do
+    Core.checkSystem "FiboWidget"
+    while !(← s.pending.anyM (IO.hasFinished ·.2)) do
+      IO.sleep 10
+      Core.checkSystem "FiboWidget"
+    let s ← s.update
+    if s.pending.isEmpty then
+      return .last <| s.render ((← IO.monoMsNow) - t0)
+    else
+      return .cont s.render (loop t0 s)
+
+-- #html FiboWidget
